Initial merging

Strata/Languages/Boogie/StatementSemantics.lean
@@ -10,6 +10,8 @@
 import Strata.DL.Imperative.CmdSemantics
 import Strata.DL.Imperative.StmtSemantics
 import Strata.DL.Imperative.HasVars
+import Strata.DL.Util.Nodup
+import Strata.DL.Util.ListUtils
 import Strata.Languages.Boogie.Procedure
 import Strata.Languages.Boogie.Statement
 import Strata.Languages.Boogie.OldExpressions
@@ -98,9 +100,9 @@ inductive UpdateStates : SemanticStore P → List P.Ident → List P.Expr → Se
     UpdateStates σ (x :: xs) (v :: vs) σ''
 
 inductive InitStates : SemanticStore P → List P.Ident → List P.Expr → SemanticStore P → Prop where
-  | update_none :
+  | init_none :
     InitStates σ [] [] σ
-  | update_some :
+  | init_some :
     InitState P σ x v σ' →
     InitStates σ' xs vs σ'' →
     InitStates σ (x :: xs) (v :: vs) σ''
@@ -199,10 +201,11 @@ inductive EvalCommand : (String → Option Procedure)  → BoogieEval → Boogie
   Here's a Zulip thread that can shed some light on this error message:
   https://leanprover-community.github.io/archive/stream/270676-lean4/topic/nested.20inductive.20datatypes.20parameters.20cannot.20contain.20local.20v.html
   -/
-  | call_sem {π δ σ₀ σ args vals σA σAO δP σR n p modvals lhs σ'} :
+  | call_sem {π δ σ₀ σ args vals oVals σA σAO δP σR n p modvals lhs σ'} :
     π n = .some p →
     EvalExpressions (P:=Expression) δ σ₀ σ args vals →
-    WellFormedSemanticEvalVal δ σ₀ σ →
+    ReadValues σ lhs oVals →
+    WellFormedSemanticEvalVal δ →
     WellFormedSemanticEvalVar δ →
     WellFormedSemanticEvalBool δ δP →
     WellFormedBoogieEvalTwoState δ σ₀ σ →
@@ -213,7 +216,9 @@ inductive EvalCommand : (String → Option Procedure)  → BoogieEval → Boogie
     -- this can't change semantics. Caller names that aren't visible to the callee won't be used. Caller
     -- names that overlap with callee names will be replaced.
     InitStates σ (Map.keys (p.header.inputs)) vals σA →
-    InitVars σA (Map.keys (p.header.outputs)) σAO →
+
+    -- need to initialize to the values of lhs, due to output variables possibly occuring in preconditions
+    InitStates σA (Map.keys (p.header.outputs)) oVals σAO →
 
     -- Preconditions, if any, must be satisfied for execution to continue.
     (∀ pre, (Procedure.Spec.getCheckExprs p.spec.preconditions).contains pre →
@@ -245,10 +250,11 @@ inductive EvalCommandContract : (String → Option Procedure)  → BoogieEval �
     ----
     EvalCommandContract π δ δP σ₀ σ (CmdExt.cmd c) σ'
 
-  | call_sem {π δ σ₀ σ args vals σA σAO σO δP σR n p modvals lhs σ'} :
+  | call_sem {π δ σ₀ σ args oVals vals σA σAO σO δP σR n p modvals lhs σ'} :
     π n = .some p →
     EvalExpressions (P:=Boogie.Expression) δ σ₀ σ args vals →
-    WellFormedSemanticEvalVal δ σ₀ σ →
+    ReadValues σ lhs oVals →
+    WellFormedSemanticEvalVal δ →
     WellFormedSemanticEvalVar δ →
     WellFormedSemanticEvalBool δ δP →
     WellFormedBoogieEvalTwoState δ σ₀ σ →
@@ -259,10 +265,9 @@ inductive EvalCommandContract : (String → Option Procedure)  → BoogieEval �
     -- this can't change semantics. Caller names that aren't visible to the callee won't be used. Caller
     -- names that overlap with callee names will be replaced.
     InitStates σ (Map.keys (p.header.inputs)) vals σA →
-    -- Q: Maybe that should be updates into value of lhs prior to call.
-    -- That would make the structure more consistent, and we will know the exact value of the store
-    -- But perhaps we don't need that
-    InitVars σA (Map.keys (p.header.outputs)) σAO →
+
+    -- need to initialize to the values of lhs, due to output variables possibly occuring in preconditions
+    InitStates σA (Map.keys (p.header.outputs)) oVals σAO →
 
     -- Preconditions, if any, must be satisfied for execution to continue.
     (∀ pre, (Procedure.Spec.getCheckExprs p.spec.preconditions).contains pre →
@@ -286,3 +291,2037 @@ abbrev EvalStatementContract (π : String → Option Procedure) : BoogieEval →
 abbrev EvalStatementsContract (π : String → Option Procedure) : BoogieEval → BoogieEvalBool →
     BoogieStore → BoogieStore → List Statement → BoogieStore → Prop :=
   Imperative.EvalStmts Expression Command (EvalCommandContract π)
+
+/-! ## Theorems -/
+
+theorem InitStatesEmpty :
+  @InitStates P σ [] [] σ' → σ = σ' := by
+  intros H; cases H <;> simp
+
+theorem UpdateStatesEmpty :
+  @UpdateStates P σ [] [] σ' → σ = σ' := by
+  intros H; cases H <;> simp
+
+theorem HavocVarsEmpty :
+  @HavocVars P σ [] σ' → σ = σ' := by
+  intros H; cases H <;> simp
+
+theorem InitVarsEmpty :
+  @InitVars P σ [] σ' → σ = σ' := by
+  intros H; cases H <;> simp
+
+theorem TouchVarsEmpty :
+  @TouchVars P σ [] σ' → σ = σ' := by
+  intros H; cases H <;> simp
+
+theorem EvalStmtsEmpty {P : PureExpr} {Cmd : Type} {EvalCmd : EvalCmdParam P Cmd}
+  { σ σ' σ₀: SemanticStore P } { δ : SemanticEval P } { δP: SemanticEvalBool P }
+  [HasVarsImp P (List (Stmt P Cmd))] [HasVarsImp P Cmd] [HasFvar P] [HasVal P] [HasBool P] [HasBoolNeg P] :
+  EvalStmts P Cmd EvalCmd δ δP σ₀ σ ([]: (List (Stmt P Cmd))) σ' → σ = σ' := by
+  intros H; cases H <;> simp
+
+theorem EvalStatementsEmpty :
+  EvalStatements π δ δP σ₀ σ [] σ' → σ = σ' := by
+  intros H; cases H <;> simp
+
+theorem EvalStatementsContractEmpty :
+  EvalStatementsContract π δ δP σ₀ σ [] σ' → σ = σ' := by
+  intros H; cases H <;> simp
+
+theorem UpdateStateNotDefMonotone
+  {P : PureExpr} {σ σ' : SemanticStore P}
+  {vs : List P.Ident} {e : P.Expr} {v : P.Ident} :
+  isNotDefined σ vs →
+  UpdateState P σ v e σ' →
+  isNotDefined σ' vs := by
+  intros Hdef Heval
+  cases Heval with
+  | update Hold HH Hsome =>
+  simp [isNotDefined] at *
+  intros v' Hv'
+  by_cases Heq: (v = v')
+  case pos =>
+    simp_all
+  case neg =>
+    specialize Hsome v' Heq
+    specialize Hdef v'
+    simp [Hsome]
+    exact Hdef Hv'
+
+theorem UpdateStatesNotDefMonotone
+  {P : PureExpr} {σ σ' : SemanticStore P}
+  {vs : List P.Ident} {es' : List P.Expr} {vs' : List P.Ident} :
+  isNotDefined σ vs →
+  UpdateStates σ vs' es' σ' →
+  isNotDefined σ' vs := by
+  intros Hdef Heval
+  induction Heval with
+  | update_none => assumption
+  | update_some Hup Hups ih =>
+  intros v Hv
+  apply ih
+  exact UpdateStateNotDefMonotone Hdef Hup
+  assumption
+
+theorem UpdateStateNotDefMonotone'
+  {P : PureExpr} {σ σ' : SemanticStore P}
+  {vs : List P.Ident} {e : P.Expr} {v : P.Ident} :
+  isNotDefined σ' vs →
+  UpdateState P σ v e σ' →
+  isNotDefined σ vs := by
+  intros Hdef Heval
+  cases Heval with
+  | update Hold HH Hsome =>
+  simp [isNotDefined] at *
+  intros v' Hv'
+  by_cases Heq: (v = v')
+  case pos =>
+    simp_all
+  case neg =>
+    specialize Hsome v' Heq
+    specialize Hdef v'
+    simp [← Hsome]
+    exact Hdef Hv'
+
+theorem UpdateStatesNotDefMonotone'
+  {P : PureExpr} {σ σ' : SemanticStore P}
+  {vs : List P.Ident} {es' : List P.Expr} {vs' : List P.Ident} :
+  isNotDefined σ' vs →
+  UpdateStates σ vs' es' σ' →
+  isNotDefined σ vs := by
+  intros Hdef Heval
+  induction Heval with
+  | update_none => assumption
+  | update_some Hup Hups ih =>
+  intros v Hv
+  apply UpdateStateNotDefMonotone' (ih Hdef) Hup
+  exact Hv
+
+theorem InitStateDefined
+  {P : PureExpr} {σ σ' : SemanticStore P} {e : P.Expr} {v : P.Ident} :
+  @InitState P σ v e σ' →
+  isDefined σ' [v] := by
+  intros Hup
+  cases Hup with
+  | init Hold Hsome Hall =>
+  simp [isDefined, Option.isSome, Hsome]
+
+theorem UpdateStateDefined
+  {P : PureExpr} {σ σ' : SemanticStore P} {e : P.Expr} {v : P.Ident} :
+  @UpdateState P σ v e σ' →
+  isDefined σ' [v] := by
+  intros Hup
+  cases Hup with
+  | update Hold Hsome Hall =>
+  simp [isDefined, Option.isSome, Hsome]
+
+theorem UpdateStateDefined'
+  {P : PureExpr} {σ σ' : SemanticStore P} {e : P.Expr} {v : P.Ident} :
+  @UpdateState P σ v e σ' →
+  isDefined σ [v] := by
+  intros Hup
+  cases Hup with
+  | update Hold Hsome Hall =>
+  simp [isDefined, Option.isSome]
+  split <;> simp_all
+
+theorem UpdateStateDefMonotone
+  {P : PureExpr} {σ σ' : SemanticStore P}
+  {vs : List P.Ident} {e : P.Expr} {v : P.Ident} :
+  isDefined σ vs →
+  UpdateState P σ v e σ' →
+  isDefined σ' vs := by
+  intros Hdef Heval
+  cases Heval with
+  | update Hold HH Hsome =>
+  simp [isDefined] at *
+  intros v' Hv'
+  by_cases Heq: (v = v')
+  case pos =>
+    simp [Option.isSome]
+    simp [Heq] at *
+    split <;> simp_all
+  case neg =>
+    specialize Hsome v' Heq
+    specialize Hdef v'
+    simp [Hsome]
+    exact Hdef Hv'
+
+theorem UpdateStatesDefMonotone
+  {P : PureExpr} {σ σ' : SemanticStore P}
+  {vs : List P.Ident} {es' : List P.Expr} {vs' : List P.Ident} :
+  isDefined σ vs →
+  UpdateStates σ vs' es' σ' →
+  isDefined σ' vs := by
+  intros Hdef Heval
+  induction Heval with
+  | update_none => assumption
+  | update_some Hup Hups ih =>
+  intros v Hv
+  apply ih
+  exact UpdateStateDefMonotone Hdef Hup
+  assumption
+
+theorem UpdateStateDefMonotone'
+  {P : PureExpr} {σ σ' : SemanticStore P}
+  {vs : List P.Ident} {e : P.Expr} {v : P.Ident} :
+  isDefined σ' vs →
+  UpdateState P σ v e σ' →
+  isDefined σ vs := by
+  intros Hdef Heval
+  cases Heval with
+  | update Hold HH Hsome =>
+  simp [isDefined] at *
+  intros v' Hv'
+  by_cases Heq: (v = v')
+  case pos =>
+    simp [Option.isSome]
+    simp [Heq] at *
+    split <;> simp_all
+  case neg =>
+    specialize Hsome v' Heq
+    specialize Hdef v'
+    simp [← Hsome]
+    exact Hdef Hv'
+
+theorem UpdateStatesDefMonotone'
+  {P : PureExpr} {σ σ' : SemanticStore P}
+  {vs : List P.Ident} {es' : List P.Expr} {vs' : List P.Ident} :
+  isDefined σ' vs →
+  UpdateStates σ vs' es' σ' →
+  isDefined σ vs := by
+  intros Hdef Heval
+  induction Heval with
+  | update_none => assumption
+  | update_some Hup Hups ih =>
+  intros v Hv
+  apply UpdateStateDefMonotone' (ih Hdef) Hup
+  exact Hv
+
+theorem UpdateStatesDefined :
+  UpdateStates σ vs es σ' →
+  isDefined σ' vs := by
+  intros Hhavoc
+  induction vs generalizing es σ σ'
+  case nil => simp [isDefined]
+  case cons h t ih =>
+    cases Hhavoc with
+    | @update_some _ _ v σ₁ _ _ Hup Hhav =>
+    apply isDefinedCons
+    apply UpdateStatesDefMonotone <;> try assumption
+    exact UpdateStateDefined Hhav
+    apply ih <;> assumption
+
+theorem UpdateStatesDefined' :
+  UpdateStates σ vs es σ' →
+  isDefined σ vs := by
+  intros Hhavoc
+  induction vs generalizing es σ σ'
+  case nil => simp [isDefined]
+  case cons h t ih =>
+    cases Hhavoc with
+    | update_some Hup Hups =>
+    apply isDefinedCons
+    exact UpdateStateDefined' Hup
+    apply UpdateStatesDefMonotone'
+    apply ih Hups
+    exact UpdateStates.update_some Hup UpdateStates.update_none
+
+theorem updatedStateUpdate {P : PureExpr}
+  {σ : SemanticStore P} {h : P.Ident} {v v' : P.Expr} :
+  σ h = some v' →
+  UpdateState P σ h v (@updatedState P σ h v) := by
+  intros Hsome
+  constructor <;> try simp [updatedState]
+  assumption
+  intros v Hneq Heq; simp_all
+
+theorem updatedStateId {P : PureExpr}
+  {σ : SemanticStore P} {h : P.Ident} {v : P.Expr} :
+  σ h = some v →
+  @updatedState P σ h v = σ := by
+  intros Hsome
+  funext x
+  simp_all [updatedState]
+
+theorem updatedStateDefMonotone :
+  isDefined σ vs →
+  isDefined (updatedState σ v' e') vs := by
+  intros Hdef
+  induction vs
+  case nil => simp [isDefined]
+  case cons h t ih =>
+    simp [isDefined] at *
+    apply And.intro
+    . simp [Option.isSome]
+      split <;> simp_all
+      next x heq =>
+      simp [updatedState] at heq
+      split at heq <;> simp_all
+    . intros id Hin
+      apply ih <;> simp_all
+
+theorem updatedStatesDefMonotone
+  {P : PureExpr} {σ : SemanticStore P}
+  {vs : List P.Ident} {ves : List (P.Ident × P.Expr)} :
+  isDefined σ vs →
+  isDefined (updatedStates' σ ves) vs := by
+  intros Hdef
+  induction ves generalizing σ <;>
+  unfold updatedStates' <;> try simp_all
+  case cons h t ih =>
+    simp [isDefined]
+    intros v Hin
+    apply ih
+    exact updatedStateDefMonotone Hdef
+    assumption
+
+  theorem updatedStatesDefined :
+  ks.length = vs.length →
+  isDefined (updatedStates σ ks vs) ks := by
+  intros Hlen k Hin
+  induction ks generalizing σ vs <;> simp_all
+  case cons h t ih =>
+  simp [updatedStates] at *
+  cases vs <;> simp at Hlen
+  case cons h' t' =>
+  cases Hin with
+  | inl Hin =>
+    simp [updatedStates']
+    have Hdef : isDefined (updatedStates' (updatedState σ h h') (t.zip t')) [h] := by
+      apply updatedStatesDefMonotone
+      simp [isDefined, updatedState]
+    simp_all [isDefined]
+  | inr Hin =>
+    apply ih <;> assumption
+
+theorem updatedStatesUpdate {P : PureExpr}
+  {σ : SemanticStore P} {hs : List P.Ident} {vs : List P.Expr} :
+  hs.length = vs.length →
+  isDefined σ hs →
+  UpdateStates σ hs vs (updatedStates σ hs vs) := by
+  intros Hlen Hdef
+  induction hs generalizing vs σ
+  case nil =>
+    simp_all
+    have Hemp : vs = [] := by
+      exact List.length_eq_zero_iff.mp (id (Eq.symm Hlen))
+    simp [Hemp, updatedStates]
+    exact UpdateStates.update_none
+  case cons h t ih =>
+    induction vs <;> simp_all
+    case cons h' t' =>
+    simp [isDefined] at Hdef
+    have Hlkup := Hdef.1
+    simp [Option.isSome] at Hlkup
+    split at Hlkup <;> simp_all
+    next x val heq =>
+    apply UpdateStates.update_some (updatedStateUpdate heq)
+    exact ih rfl (updatedStateDefMonotone Hdef)
+
+theorem updatedStateInit {P : PureExpr}
+  {σ : SemanticStore P} {h : P.Ident} {v : P.Expr} :
+  σ h = none →
+  InitState P σ h v (@updatedState P σ h v) := by
+  intros Hsome
+  constructor <;> try simp [updatedState]
+  assumption
+  intros v Hneq Heq; simp_all
+
+theorem updatedStatesInit {P : PureExpr}
+  {σ : SemanticStore P} {hs : List P.Ident} {vs : List P.Expr} :
+  hs.length = vs.length →
+  isNotDefined σ hs →
+  hs.Nodup →
+  InitStates σ hs vs (updatedStates σ hs vs) := by
+  intros Hlen Hdef Hnd
+  induction hs generalizing vs σ
+  case nil =>
+    simp_all
+    have Hemp : vs = [] := by
+      exact List.length_eq_zero_iff.mp (id (Eq.symm Hlen))
+    simp [Hemp, updatedStates]
+    exact InitStates.init_none
+  case cons h t ih =>
+    induction vs <;> simp_all
+    case cons h' t' =>
+    simp [isNotDefined] at Hdef
+    have Hlkup := Hdef.1
+    simp at Hlkup
+    apply InitStates.init_some (updatedStateInit Hlkup)
+    apply ih rfl
+    simp [isNotDefined, updatedState]
+    intros v Hin
+    simp_all
+    exact ne_of_mem_of_not_mem Hin Hnd.1
+
+/-- use the zipped version to avoid needing to prove length equivalent -/
+theorem updatedStates'App :
+  updatedStates' σ (a ++ b) =
+  updatedStates' (updatedStates' σ a) b := by
+  induction a generalizing σ
+  case nil =>
+    simp [updatedStates']
+  case cons h t ih =>
+    simp [updatedStates']
+    rw [ih]
+
+theorem InitStatesInitVars :
+  InitStates σ hs vs σ' →
+  InitVars σ hs σ' := by
+  intros Hinit
+  induction Hinit
+  case init_none => exact InitVars.init_none
+  case init_some h t ih => exact InitVars.init_some h ih
+
+theorem InitStatesInits :
+  InitStates σ hs vs σ' →
+  Inits σ σ' := by
+  intros Hinit
+  constructor
+  exact InitStatesInitVars Hinit
+
+theorem InitStatesNotDefined :
+  InitStates σ hs vs σ' → isNotDefined σ hs := by
+  intros Hinit
+  induction Hinit <;> simp [isNotDefined]
+  case init_some x v σ' xs vs σ'' Hinit Hinits ih =>
+    simp [isNotDefined] at *
+    cases Hinit with
+    | init Hnone Hsome Heq =>
+    refine ⟨Hnone, ?_⟩
+    intros x' Hin
+    by_cases Heqx : x = x' <;> simp_all
+    specialize Heq x' Heqx
+    specialize ih x' Hin
+    simp_all
+
+theorem InitStatesNodup :
+  InitStates σ hs vs σ' → hs.Nodup := by
+  intros Hinit
+  induction Hinit <;> simp_all
+  case init_some x v σ' xs vs σ'' Hinit Hinits ih =>
+  apply Not.intro
+  intros Hin
+  cases Hinit with
+  | init Hnone Hsome Heq =>
+    have Hnd := InitStatesNotDefined Hinits
+    specialize Hnd x Hin
+    simp_all
+
+theorem InitStateInjective :
+  InitState P σ k1 k2 σ' →
+  InitState P σ k1 k2 σ'' →
+  σ' = σ'' := by
+  intros Hinit1 Hinit2
+  cases Hinit1
+  case init Hnone1 Heq1 Hsome1 =>
+  cases Hinit2
+  case init Hnone2 Heq2 Hsome2 =>
+  funext x
+  by_cases H : k1 = x
+  . simp_all
+  . rw [Heq1, Heq2] <;> simp_all
+
+theorem InitStatesInjective :
+  InitStates σ k1 k2 σ' →
+  InitStates σ k1 k2 σ'' →
+  σ' = σ'' := by
+  intros Hinit1 Hinit2
+  induction Hinit1 generalizing σ''
+  case init_none =>
+    have Heq := InitStatesEmpty Hinit2
+    simp_all
+  case init_some Hinit Hinits ih =>
+    cases Hinit2 with
+    | init_some Hinit2 Hinits2 =>
+    apply ih
+    have Hinj := InitStateInjective Hinit Hinit2
+    simp_all
+
+theorem ReadValuesInjective :
+  ReadValues σ ks vs →
+  ReadValues σ ks vs' →
+  vs = vs' := by
+  intros Hrd1 Hrd2
+  induction Hrd1 generalizing vs'
+  case read_none =>
+    cases Hrd2
+    rfl
+  case read_some Hrd Hrds ih =>
+    cases Hrd2 with
+    | read_some Hrd2 Hrds2 =>
+    congr
+    . simp_all
+    . apply ih
+      simp_all
+
+theorem InitStateUpdated :
+    InitState P σ' k v σ'' →
+    σ'' = updatedState σ' k v := by
+  intros Hinit
+  cases Hinit with
+  | init Hnone Hsome Heq =>
+  funext x
+  simp [updatedState]
+  by_cases Hxk : x = k <;> simp_all
+  rw [Heq]
+  exact fun a => Hxk (Eq.symm a)
+
+theorem InitStatesUpdated :
+    InitStates σ' ks vs σ'' →
+    σ'' = updatedStates σ' ks vs := by
+  intros Hinit
+  induction Hinit
+  case init_none =>
+    simp [updatedStates, updatedStates']
+  case init_some Hinit Hinits ih =>
+    simp [ih]
+    simp [updatedStates, updatedStates']
+    have Heq := InitStateUpdated Hinit
+    simp [Heq]
+
+theorem UpdateStateUpdated :
+    UpdateState P σ' k v σ'' →
+    σ'' = updatedState σ' k v := by
+  intros Hinit
+  cases Hinit with
+  | update Hnone Hsome Heq =>
+  funext x
+  simp [updatedState]
+  by_cases Hxk : x = k <;> simp_all
+  rw [Heq]
+  exact fun a => Hxk (Eq.symm a)
+
+theorem UpdateStatesUpdated :
+    UpdateStates σ' ks vs σ'' →
+    σ'' = updatedStates σ' ks vs := by
+  intros Hinit
+  induction Hinit
+  case update_none =>
+    simp [updatedStates, updatedStates']
+  case update_some Hinit Hinits ih =>
+    simp [ih]
+    simp [updatedStates, updatedStates']
+    have Heq := UpdateStateUpdated Hinit
+    simp [Heq]
+
+theorem InitStatesApp' :
+  InitStates σ (k1 ++ k2) (v1 ++ v2) σ' →
+  k1.length = v1.length →
+  k2.length = v2.length →
+  ∃ σ₁,
+  σ₁ = updatedStates σ k1 v1 ∧
+  InitStates σ k1 v1 σ₁ ∧
+  InitStates σ₁ k2 v2 σ' := by
+  intros Hinit Hlen1 Hlen2
+  exists (updatedStates σ k1 v1)
+  refine ⟨rfl, ?_⟩
+  have H1 : InitStates σ k1 v1 (updatedStates σ k1 v1) := by
+    apply updatedStatesInit Hlen1
+    . have Hndef := InitStatesNotDefined Hinit
+      simp [isNotDefined] at *
+      simp_all
+    . have Hndup := InitStatesNodup Hinit
+      refine List.Sublist.nodup ?_ Hndup
+      exact List.sublist_append_left k1 k2
+  refine ⟨H1, ?_⟩
+  generalize Hup : updatedStates σ k1 v1 = σ₁ at *
+  induction H1 <;> simp_all
+  case init_some σ₂ Hinit' Hinits ih =>
+  apply ih
+  . cases Hinit with
+    | init_some Hinit Hinits =>
+      simp [InitStateInjective Hinit Hinit'] at *
+      assumption
+  . simp [InitStateUpdated Hinit']
+    exact Hup
+
+theorem ReadValuesApp :
+  ReadValues σ k1 v1 →
+  ReadValues σ k2 v2 →
+  ReadValues σ (k1 ++ k2) (v1 ++ v2) := by
+  intros Hrd1 Hrd2
+  induction Hrd1 <;> simp_all
+  case read_some Hsome Hrd Hrds =>
+  constructor <;> assumption
+
+theorem ReadValuesAppKeys' :
+  ReadValues σ (k1 ++ k2) vs →
+  exists v1 v2,
+  v1 ++ v2 = vs ∧
+  ReadValues σ k1 v1 ∧
+  ReadValues σ k2 v2 := by
+  intros Hrd
+  induction vs generalizing k1 k2
+  case nil =>
+    exists [],[]
+    generalize Hk12 : k1 ++ k2 = k12 at Hrd
+    cases Hrd
+    simp_all
+    constructor
+  case cons vh vt vih =>
+    cases k1
+    case nil =>
+      exists [],vh :: vt
+      simp_all
+      constructor
+    case cons kh kt =>
+      cases Hrd with
+      | read_some Hsome Hrd =>
+        specialize vih Hrd
+        cases vih with
+        | intro v1' vih =>
+        cases vih with
+        | intro v2 vih =>
+        exists vh::v1',v2
+        simp_all
+        constructor <;> simp_all
+
+theorem ReadValuesLength :
+  ReadValues σ ks vs →
+  ks.length = vs.length := by
+  intros Hrd
+  induction Hrd <;> simp_all
+
+theorem EvalExpressionsLength :
+  EvalExpressions (P:=Boogie.Expression) δ σ σ₀ ks vs →
+  ks.length = vs.length := by
+  intros Hrd
+  induction Hrd <;> simp_all
+
+theorem InitStatesLength :
+  InitStates σ ks vs σ' →
+  ks.length = vs.length := by
+  intros Hinit
+  induction Hinit <;> simp_all
+
+theorem UpdateStatesLength {P : PureExpr}
+  {σ σ' : Imperative.SemanticStore P}
+  {ks : List P.Ident}
+  {vs : List P.Expr}
+  :
+  UpdateStates (P:=P) σ ks vs σ' →
+  List.length ks = List.length vs := by
+  intros Hup
+  induction Hup <;> simp_all
+
+theorem InitStateReadValuesMonotone {P : PureExpr} {σ σ' : SemanticStore P}
+  {ks : List P.Ident} {vs : List P.Expr} {e : P.Expr} {v : P.Ident} :
+  ReadValues σ ks vs →
+  InitState P σ v e σ' →
+  ReadValues σ' ks vs := by
+  intros Hdef Heval
+  cases Heval with
+  | init Hold HH Hsome =>
+  induction Hdef
+  case read_none => constructor
+  case read_some xs vs' x v' Hsome' Hrd Hrds =>
+  constructor <;> simp_all
+  rw [Hsome] <;> try simp_all
+  apply Not.intro
+  intros Heq
+  simp_all
+
+theorem InitStatesReadValuesMonotone
+  {P : PureExpr} {σ σ' : SemanticStore P}
+  {ks : List P.Ident} {vs : List P.Expr}
+  {es' : List P.Expr} {vs' : List P.Ident} :
+  ReadValues σ ks vs →
+  InitStates σ vs' es' σ' →
+  ReadValues σ' ks vs := by
+  intros Hdef Heval
+  induction Heval with
+  | init_none => assumption
+  | init_some Hinit Hinits ih =>
+    apply ih
+    apply InitStateReadValuesMonotone <;> assumption
+
+theorem UpdateStateReadValuesMonotone {P : PureExpr} {σ σ' : SemanticStore P}
+  {ks : List P.Ident} {vs : List P.Expr} {e : P.Expr} {v : P.Ident} :
+  ¬ v ∈ ks →
+  ReadValues σ ks vs →
+  UpdateState P σ v e σ' →
+  ReadValues σ' ks vs := by
+  intros Hnin Hdef Heval
+  cases Heval with
+  | update Hold HH Hsome =>
+  induction Hdef
+  case read_none => constructor
+  case read_some xs vs' x v' Hsome' Hrd Hrds =>
+  constructor <;> simp_all
+
+theorem UpdateStatesReadValuesMonotone
+  {P : PureExpr} {σ σ' : SemanticStore P}
+  {ks : List P.Ident} {vs : List P.Expr}
+  {es' : List P.Expr} {vs' : List P.Ident} :
+  (ks ++ vs').Nodup →
+  ReadValues σ ks vs →
+  UpdateStates σ vs' es' σ' →
+  ReadValues σ' ks vs := by
+  intros Hnd Hdef Heval
+  induction Heval with
+  | update_none => assumption
+  | update_some Hinit Hinits ih =>
+    have Hnd' := nodup_middle Hnd
+    simp_all
+    apply ih
+    apply UpdateStateReadValuesMonotone _ Hdef Hinit <;> try assumption
+    simp_all
+
+theorem InitStateReadValues :
+  InitState P σ v e σ' →
+  ReadValues σ' [v] [e] := by
+  intros Hinit
+  cases Hinit with
+  | init Hold HH Hsome =>
+  constructor
+  . assumption
+  . constructor
+
+theorem UpdateStateReadValues :
+  UpdateState P σ v e σ' →
+  ReadValues σ' [v] [e] := by
+  intros Hinit
+  cases Hinit with
+  | update Hold HH Hsome =>
+  constructor
+  . assumption
+  . constructor
+
+theorem InitStatesReadValues :
+  InitStates σ vs es σ' →
+  ReadValues σ' vs es := by
+  intros Hinit
+  induction Hinit
+  case init_none =>
+    constructor
+  case init_some x v σ₁ x' v' σ'' Hinit Hinits ih =>
+    constructor <;> try assumption
+    have Hrd : ReadValues σ'' [x] [v] := by
+      apply InitStatesReadValuesMonotone (σ:=σ₁)
+      apply InitStateReadValues <;> assumption
+      assumption
+    cases Hrd
+    assumption
+
+theorem UpdateStatesReadValues :
+  vs.Nodup →
+  UpdateStates σ vs es σ' →
+  ReadValues σ' vs es := by
+  intros Hnd Hinit
+  induction Hinit
+  case update_none =>
+    constructor
+  case update_some x v σ₁ x' v' σ'' Hupdate Hupdates ih =>
+    constructor <;> try assumption
+    have Hrd : ReadValues σ'' [x] [v] := by
+      apply UpdateStatesReadValuesMonotone (σ:=σ₁)
+      exact Hnd
+      apply UpdateStateReadValues <;> assumption
+      assumption
+    cases Hrd
+    assumption
+    apply ih
+    simp_all
+
+theorem InitVarsInitStates : InitVars σ vars σ' →
+  ∃ modvals, InitStates σ vars modvals σ' := by
+  intros Hinit
+  induction Hinit
+  case init_none =>
+    refine ⟨[], InitStates.init_none⟩
+  case init_some σ x v σ₁ xs σ'' Hup Hhav ih =>
+    cases ih with
+    | intro vs Hups =>
+    refine ⟨v::vs,?_⟩
+    constructor <;> assumption
+
+theorem InitVarsReadValuesMonotone
+  {P : PureExpr} {σ σ' : SemanticStore P}
+  {ks vs' : List P.Ident} {vs : List P.Expr} :
+  ReadValues σ ks vs →
+  InitVars σ vs' σ' →
+  ReadValues σ' ks vs := by
+  intros Hdef Hinit
+  have Hinit' := InitVarsInitStates Hinit
+  cases Hinit' with
+  | intro es' Hinit' =>
+  exact InitStatesReadValuesMonotone Hdef Hinit'
+
+theorem updatedStateComm
+  {P : PureExpr} {σ : SemanticStore P}
+  {k k' : P.Ident} {v v' : P.Expr} :
+  k ≠ k' →
+  updatedState (updatedState σ k v) k' v' =
+  updatedState (updatedState σ k' v') k v := by
+  intros Hne
+  funext x
+  unfold updatedState
+  by_cases Hxk' : x = k' <;> simp [Hxk']
+  intros Heq
+  by_cases Hxk : x = k <;> simp_all
+
+theorem updatedStateComm'
+  {P : PureExpr} {σ : SemanticStore P}
+  {k : P.Ident} {v : P.Expr}
+  {kvs : List (P.Ident × P.Expr)} :
+  ¬ k ∈ kvs.unzip.1 →
+  (updatedState (updatedStates' σ kvs) k v) =
+  (updatedStates' (updatedState σ k v) kvs) := by
+  intros Hnd
+  induction kvs generalizing σ <;> simp [updatedStates']
+  case cons h t ih =>
+  rw [ih]
+  rw [updatedStateComm]
+  simp_all; exact fun a => Hnd.1 (Eq.symm a)
+  simp_all
+
+theorem updatedStatesComm
+  {P : PureExpr} {σ : SemanticStore P}
+  {kvs kvs' : List (P.Ident × P.Expr)} :
+  kvs.unzip.1.Disjoint kvs'.unzip.1 →
+  updatedStates' (updatedStates' σ kvs) kvs' =
+  updatedStates' (updatedStates' σ kvs') kvs := by
+  intros Hnd
+  induction kvs generalizing kvs' σ <;> simp [updatedStates']
+  case cons h t ih =>
+  induction kvs' generalizing σ h <;> simp [updatedStates']
+  case cons h' t' ih' =>
+    rw [← ih']
+    rw [updatedStateComm]
+    rw [updatedStateComm']
+    . simp at Hnd
+      have Hnd' := List.Disjoint.symm Hnd
+      apply List.Disjoint_cons_head
+      apply List.Disjoint.mono_right _ Hnd'
+      simp_all
+    . intros Hin
+      simp_all [List.Disjoint]
+    . simp at *
+      refine List.Disjoint.mono_right ?_ Hnd
+      simp_all
+
+theorem UpdateStateSomeMonotone
+  {P : PureExpr} {σ σ' : SemanticStore P}
+  {k' : P.Ident} {v' : P.Expr} {e : P.Expr} {v : P.Ident} :
+  v ≠ k' →
+  σ k' = some v' →
+  UpdateState P σ v e σ' →
+  σ' k' = some v' := by
+  intros Hne Hdef Heval
+  have Hrd : ReadValues σ [k'] [v'] := by
+    cases Heval with
+    | update Hold HH Hsome =>
+    constructor <;> simp_all
+    constructor
+  have Hrd2 : ReadValues σ' [k'] [v'] := by
+    apply UpdateStateReadValuesMonotone ?_ Hrd Heval
+    simp_all
+  cases Hrd2
+  assumption
+
+theorem UpdateStatesSomeMonotone
+  {P : PureExpr} {σ σ' : SemanticStore P}
+  {k' : P.Ident} {v' : P.Expr}
+  {ks': List P.Ident} {vs': List P.Expr} :
+  ¬ k' ∈ ks' →
+  σ k' = some v' →
+  UpdateStates σ ks' vs' σ' →
+  σ' k' = some v' := by
+  intros Hnin Hsome Hinit
+  induction Hinit <;> try simp_all
+  next Hinit Hinits ih =>
+  apply ih
+  apply UpdateStateSomeMonotone ?_ Hsome Hinit
+  exact fun a => Hnin.1 (Eq.symm a)
+
+theorem InitStateSomeMonotone
+  {P : PureExpr} {σ σ' : SemanticStore P}
+  {k' : P.Ident} {v' : P.Expr} {e : P.Expr} {v : P.Ident} :
+  σ k' = some v' →
+  InitState P σ v e σ' →
+  σ' k' = some v' := by
+  intros Hdef Heval
+  have Hrd : ReadValues σ [k'] [v'] := by
+    cases Heval with
+    | init Hold HH Hsome =>
+    constructor <;> simp_all
+    constructor
+  have Hrd2 : ReadValues σ' [k'] [v'] :=
+    InitStateReadValuesMonotone Hrd Heval
+  cases Hrd2
+  assumption
+
+theorem InitStateSomeMonotone'
+  {P : PureExpr} {σ σ' : SemanticStore P}
+  {k' : P.Ident} {v' : P.Expr} {e : P.Expr} {v : P.Ident} :
+  k' ≠ v →
+  σ' k' = some v' →
+  InitState P σ v e σ' →
+  σ k' = some v' := by
+  intros Hne Hdef Heval
+  have Hrd : ReadValues σ [k'] [v'] := by
+    cases Heval with
+    | init Hold HH Hsome =>
+    constructor <;> simp_all
+    rw [← Hsome]
+    assumption
+    exact fun a => Hne (Eq.symm a)
+    constructor
+  have Hrd2 : ReadValues σ' [k'] [v'] :=
+    InitStateReadValuesMonotone Hrd Heval
+  cases Hrd
+  assumption
+
+theorem InitStatesSomeMonotone
+  {P : PureExpr} {σ σ' : SemanticStore P}
+  {k' : P.Ident} {v' : P.Expr}
+  {ks': List P.Ident} {vs': List P.Expr} :
+  σ k' = some v' →
+  InitStates σ ks' vs' σ' →
+  σ' k' = some v' := by
+  intros Hsome Hinit
+  induction Hinit <;> try simp_all
+  next Hinit Hinits ih =>
+  apply ih
+  apply InitStateSomeMonotone Hsome Hinit
+
+theorem InitStatesSomeMonotone'
+  {P : PureExpr} {σ σ' : SemanticStore P}
+  {k' : P.Ident} {v' : P.Expr}
+  {ks': List P.Ident} {vs': List P.Expr} :
+  ¬ k' ∈ ks' →
+  σ' k' = some v' →
+  InitStates σ ks' vs' σ' →
+  σ k' = some v' := by
+  intros Hnin Hsome Hinit
+  induction Hinit
+  case init_none => simp_all
+  case init_some Hinit Hinits ih =>
+  apply InitStateSomeMonotone' ?_ ?_ Hinit
+  . simp_all
+  . apply ih <;> simp_all
+
+theorem InitsUpdatesComm
+  {P : PureExpr} {σ σ' σ'' : SemanticStore P}
+  {ks ks' : List P.Ident} {vs vs' : List P.Expr} :
+  UpdateStates σ ks vs σ' →
+  InitStates σ' ks' vs' σ'' →
+  ∃ σ₁,
+    σ₁ = (updatedStates σ ks' vs') ∧
+    InitStates σ ks' vs' σ₁ ∧
+    UpdateStates σ₁ ks vs σ'' := by
+  intros Hup Hinit
+  exists (updatedStates σ ks' vs')
+  have Hk : (isDefined σ' ks) := UpdateStatesDefined Hup
+  have Hlen1 := InitStatesLength Hinit
+  have Hlen2 := UpdateStatesLength Hup
+  induction Hup generalizing σ''
+  case update_none =>
+    simp_all
+    apply And.intro
+    refine updatedStatesInit Hlen1 ?_ ?_
+    exact InitStatesNotDefined Hinit
+    exact InitStatesNodup Hinit
+    simp [InitStatesUpdated Hinit]
+    constructor
+  case update_some σ x v σ₀ xs vs σ₁ Hup Hups ih =>
+    refine ⟨rfl, ?_, ?_⟩
+    . apply updatedStatesInit Hlen1
+      apply UpdateStateNotDefMonotone' ?_ Hup
+      apply UpdateStatesNotDefMonotone' ?_ Hups
+      exact InitStatesNotDefined Hinit
+      exact InitStatesNodup Hinit
+    . apply UpdateStates.update_some (σ':=updatedStates σ₀ ks' vs')
+      . simp [UpdateStateUpdated Hup, updatedStates]
+        rw [← updatedStateComm']
+        . have Hdef := UpdateStateDefined' Hup
+          simp [isDefined, Option.isSome] at Hdef
+          split at Hdef <;> simp_all
+          next val heq =>
+          apply updatedStateUpdate (v':=val)
+          apply InitStatesSomeMonotone heq
+          apply updatedStatesInit
+          . simp_all
+          . apply UpdateStateNotDefMonotone' ?_ Hup
+            apply UpdateStatesNotDefMonotone' ?_ Hups
+            apply InitStatesNotDefined Hinit
+          . exact InitStatesNodup Hinit
+        . rw [List.unzip_zip] <;> simp_all
+          have Hnd := InitStatesNotDefined Hinit
+          simp [isNotDefined, isDefined] at *
+          apply Not.intro
+          intros Hin
+          specialize Hnd _ Hin
+          simp_all
+      . apply (ih Hinit ?_ ?_).2.2
+        . simp [isDefined] at * <;> simp_all
+        . simp_all
+
+theorem InitUpdateComm
+  {P : PureExpr} {σ σ' σ'' : SemanticStore P}
+  {k k' : P.Ident} {v v' : P.Expr}
+  :
+  UpdateState P σ k v σ' →
+  InitState P σ' k' v' σ'' →
+  ∃ σ₁,
+    σ₁ = (updatedState σ k' v') ∧
+    InitState P σ k' v' σ₁ ∧
+    UpdateState P σ₁ k v σ'' := by
+  intros Hup Hinit
+  exists (updatedState σ k' v')
+  have Hk : (isDefined σ' [k]) := UpdateStateDefined Hup
+  have Hups : UpdateStates σ [k] [v] σ' := by
+    apply UpdateStates.update_some Hup UpdateStates.update_none
+  have Hinits : InitStates σ' [k'] [v'] σ'' := by
+    apply InitStates.init_some Hinit InitStates.init_none
+  have Hcomms := InitsUpdatesComm Hups Hinits
+  simp at Hcomms
+  refine ⟨rfl, ?_, ?_⟩
+  . have Hinit := Hcomms.1
+    cases Hinit with
+    | init_some Hinit Hinits =>
+    simp [InitStatesEmpty Hinits, updatedStates, updatedStates'] at Hinit
+    assumption
+  . have Hup := Hcomms.2
+    cases Hup with
+    | update_some Hup Hups =>
+    simp [UpdateStatesEmpty Hups, updatedStates, updatedStates'] at Hup
+    assumption
+
+theorem isDefinedReadValues :
+  isDefined σ ks →
+  ∃ vs,
+  ReadValues σ ks vs := by
+  intros Hdef
+  simp [isDefined] at Hdef
+  induction ks <;> simp_all
+  case nil =>
+    exists []
+    constructor
+  case cons h t ih =>
+    cases ih with
+    | intro t' Hrd =>
+    have Hsome := Hdef.1
+    simp [Option.isSome] at Hsome
+    split at Hsome <;> simp_all
+    next h' Hh' =>
+    exists (h' :: t')
+    constructor <;> simp_all
+
+theorem ReadValuesIsDefined :
+  ReadValues σ ks vs →
+  isDefined σ ks := by
+  intros Hrd
+  induction Hrd <;> simp [isDefined, Option.isSome]
+  apply And.intro
+  . split <;> simp_all
+  . intros a Hin
+    split <;> simp_all
+    next ih ex Hnone =>
+    specialize ih a Hin
+    simp_all
+
+theorem InitStateSubstStores :
+σ k' = some v' →
+InitState Expression σ k v' σ' →
+substStores σ σ' [(k', k)] := by
+intros Hsome Hinit
+cases Hinit with
+| init Hone Hsome' Heq =>
+simp [substStores]
+simp [Hsome, Hsome']
+
+theorem InitStatesSubstStores :
+ReadValues σ ks' vs' →
+InitStates σ ks vs' σ' →
+substStores σ σ' (ks'.zip ks) := by
+intros Hrd Hinit
+induction Hinit generalizing ks' with
+| init_none =>
+  simp [substStores]
+| init_some Hinit Hinits ih =>
+  next σ x v σ₁ xs vs σ'' =>
+  cases Hrd with
+  | read_some Hsome'' Hrds =>
+  next ys y =>
+  have Hinit' := Hinit
+  cases Hinit with
+  | init Hnone Hsome' Heq =>
+  simp [substStores]
+  intros k1 k2 Hin
+  cases Hin with
+  | inl Hin =>
+    simp_all
+    apply Eq.symm
+    apply InitStatesSomeMonotone Hsome' Hinits
+  | inr Hin =>
+    specialize @ih ys ?_
+    exact InitStateReadValuesMonotone Hrds Hinit'
+    rw [← Heq]
+    exact ih k1 k2 Hin
+    apply Not.intro
+    intro Heq
+    simp_all
+    have Hin' := List.of_mem_zip Hin
+    have Hdef := ReadValuesIsDefined Hrds
+    specialize Hdef k1 Hin'.1
+    simp_all
+
+theorem substStoresInitInv :
+substDefined σ σ' substs →
+substStores σ σ' substs →
+InitState Expression σ' k v σ'' →
+substStores σ σ'' substs := by
+intros Hdef Hsubst Hinit
+simp [substStores, substDefined] at *
+intros k1 k2 Hin
+cases Hinit with
+| init Hnone Hsome' Heq =>
+rw [Heq] <;> simp_all
+rw [Hsubst] <;> simp_all
+apply Not.intro
+intro Heq'
+simp [Heq'] at *
+specialize Hdef k1 k2 Hin
+simp [Option.isSome] at Hdef
+split at Hdef <;> simp_all
+
+theorem substStoresInitsInv :
+substDefined σ σ' substs →
+substStores σ σ' substs →
+InitStates σ' ks vs σ'' →
+substStores σ σ'' substs := by
+intros Hdef Hsubst Hinit
+simp [substStores, substDefined] at *
+intros k1 k2 Hin
+induction Hinit generalizing σ
+case init_none =>
+  exact Hsubst k1 k2 Hin
+case init_some Hinit Hinits ih =>
+  simp [Hsubst k1 k2 Hin]
+  specialize Hdef k1 k2 Hin
+  simp [Option.isSome] at Hdef
+  split at Hdef <;> simp_all
+  split at Hdef <;> simp_all
+  next x val Hsome =>
+  have Hsome' := InitStateSomeMonotone Hsome Hinit
+  have Hsome'' := InitStatesSomeMonotone Hsome' Hinits
+  simp_all
+
+theorem substStoresInitsInv' :
+substDefined σ σ' substs →
+substStores σ σ' substs →
+InitStates σ ks vs σ'' →
+substStores σ'' σ' substs := by
+  intros k1 k2 Hin
+  rw [← substSwapId _ substs]
+  apply substStoresFlip
+  apply substStoresInitsInv <;> try assumption
+  . exact substDefinedFlip k1
+  . exact substStoresFlip k2
+
+theorem substStoresUpdateInv {k : P.Ident} {substs : List (P.Ident × P.Ident)}:
+¬ k ∈ substs.unzip.2 →
+substStores (P:=P) σ σ' substs →
+UpdateState (P:=P) σ' k v σ'' →
+substStores (P:=P) σ σ'' substs := by
+intros Hnin Hsubst Hinit
+simp [substStores] at *
+intros k1 k2 Hin
+cases Hinit with
+| update Hnone Hsome' Heq =>
+rw [Heq] <;> simp_all
+rw [Hsubst] <;> simp_all
+intros Heq'
+specialize Hnin k1
+simp_all
+
+theorem substStoresUpdatesInv :
+ks.Disjoint substs.unzip.2 →
+substStores σ σ' substs →
+UpdateStates σ' ks vs σ'' →
+substStores σ σ'' substs := by
+intros Hnin Hsubst Hup
+simp [substStores] at *
+intros k1 k2 Hin
+induction Hup generalizing σ
+case update_none =>
+  exact Hsubst k1 k2 Hin
+case update_some σ x v σ' xs vs σ₁ Hup Hinits ih =>
+  have Hnin : ¬ x ∈ substs.unzip.2 := by
+    simp [List.Disjoint] at Hnin
+    intros Hin
+    have Hprod := List.mem_zip_2 (l₁:=substs.unzip.fst) (by simp) Hin
+    rw [List.zip_unzip] at Hprod
+    cases Hprod with
+    | intro w Hprod =>
+    have HH := Hnin.1 w
+    contradiction
+  have HH := substStoresUpdateInv (σ:=σ) Hnin Hsubst Hup
+  apply ih HH
+  simp [List.Disjoint] at *
+  simp_all
+
+theorem substStoresUpdatesInv' :
+ks.Disjoint substs.unzip.1 →
+substStores σ σ' substs →
+UpdateStates σ ks vs σ'' →
+substStores σ'' σ' substs := by
+  intros Hdisj Hsubst Hup
+  rw [← substSwapId _ substs]
+  apply substStoresFlip
+  apply substStoresUpdatesInv <;> try assumption
+  . intros a Hin Hin'
+    specialize Hdisj Hin
+    simp [substSwap] at Hin'
+    simp_all
+  . exact substStoresFlip Hsubst
+
+theorem substDefinedIsDefined :
+  substDefined σ σ' substs →
+  isDefined σ substs.unzip.1 ∧
+  isDefined σ' substs.unzip.2 := by
+  intros Hsubst
+  cases substs <;> simp [isDefined, substDefined] at *
+  case cons h t =>
+    apply And.intro
+    . apply And.intro
+      . exact (Hsubst h.1 h.2 (Or.inl rfl)).1
+      . intros k1 k2 Hin
+        exact (Hsubst k1 k2 (Or.inr Hin)).1
+    . apply And.intro
+      . exact (Hsubst h.1 h.2 ((Or.inl rfl))).2
+      . intros k2 k1 Hin
+        exact (Hsubst k1 k2 (Or.inr Hin)).2
+
+/--
+We require substNodup on keys here, because
+if we want σ [(x, y), (y, z)] σ' by constructing σ' from σ
+there are two ways:
+1. σ₁ := σ [y → x], σ' := σ₁ [z → y]. This way, z = σ(x) in σ'
+2. σ₁ := σ [z → y], σ' := σ₁ [y → x]. This way, z = σ(y) in σ'
+This creates ambiguity when we deterministically compute the substitution.
+It is more common to assume commutativity of substitution, meaning it stays non-order sensitive.
+This is why Nodup is included as a part of substStores
+-/
+theorem substStoresCons' :
+  substNodup ((h,h') :: substs) →
+  substDefined σ σ'' ((h,h') :: substs) →
+  substStores σ σ'' ((h,h') :: substs) →
+  ∃ σ' v,
+    σ h = some v ∧
+    σ' = updatedState σ h' v ∧
+    substStores σ σ' [(h,h')] ∧
+    substStores σ' σ'' substs := by
+  intros Hnd Hdef Hsubst
+  simp [substStores, substDefined] at *
+  have Hsome : (σ h).isSome = true := by
+    simp [Option.isSome]
+    specialize Hdef h h'
+    split <;> simp_all
+  cases Hh: σ h with
+  | none =>
+    exfalso
+    specialize Hdef h h'
+    simp_all
+  | some v =>
+    exists (updatedState σ h' v)
+    simp [updatedState]
+    simp [substNodup] at Hnd
+    intros k1 k2 Hin
+    split <;> simp_all
+    next heq =>
+      have Hnd' := Hnd.2
+      have Hin' : h' ∈ substs.unzip.1 := by
+        simp_all
+        exists k2
+      exfalso
+      have Hnd' := nodup_middle Hnd'
+      simp_all
+    next hne =>
+      apply Hsubst
+      exact Or.inr Hin
+
+theorem substStoresCons :
+  substStores σ σ' [(h,h')] →
+  substStores σ σ' (List.zip t t') →
+  substStores σ σ' ((h,h') :: (List.zip t t')) := by
+  intros Hh Ht
+  intros k1 k2 Hin
+  simp at Hin
+  cases Hin with
+  | inl Hin =>
+    apply Hh
+    simp_all
+  | inr Hin =>
+    apply Ht
+    simp_all
+
+theorem ReadValuesSubstStores :
+  ReadValues σ ks vs →
+  ReadValues σ' ks' vs →
+  Imperative.substStores σ σ' (List.zip ks ks') := by
+  intros H1 H2
+  induction vs generalizing ks ks'
+  case nil =>
+    cases H1
+    cases H2
+    intros h1 h2 Hin
+    cases Hin
+  case cons h t ih =>
+    cases ks
+    cases H1
+    cases ks'
+    cases H2
+    cases H1 with
+    | read_some Hh Ht =>
+    cases H2 with
+    | read_some Hh' Ht' =>
+    simp
+    apply substStoresCons
+    . simp [substStores]
+      simp_all
+    . exact ih Ht Ht'
+
+theorem EvalStatementsContractApp' :
+  EvalStatementsContract π δ δP σ₀ σ (ss₁ ++ ss₂) σ'' →
+  ∃ σ',
+    EvalStatementsContract π δ δP σ₀ σ ss₁ σ' ∧
+    EvalStatementsContract π δ δP σ₀ σ' ss₂ σ'' := by
+  intros Heval
+  induction ss₁ generalizing σ <;> simp_all
+  case nil =>
+    exists σ <;> simp_all
+    exact EvalStmts.stmts_none_sem
+  case cons h t ih =>
+    cases Heval with
+    | stmts_some_sem Hh Ht =>
+    next σ' =>
+    specialize ih Ht
+    cases ih with
+    | intro σ'' Heval =>
+    exists σ''
+    simp_all
+    exact EvalStmts.stmts_some_sem Hh Heval.1
+
+theorem EvalStatementsContractApp :
+  EvalStatementsContract π δ δP σ₀ σ ss₁ σ' →
+  EvalStatementsContract π δ δP σ₀ σ' ss₂ σ'' →
+  EvalStatementsContract π δ δP σ₀ σ (ss₁ ++ ss₂) σ'' := by
+  intros Heval1 Heval2
+  induction ss₁ generalizing σ <;> simp_all
+  case nil =>
+    simp [EvalStatementsContractEmpty Heval1]
+    assumption
+  case cons h t ih =>
+    cases Heval1 with
+    | stmts_some_sem Heval Heval' =>
+    constructor
+    . exact Heval
+    . apply ih
+      exact Heval'
+
+theorem EvalStatementsApp :
+  EvalStatements π δ δP σ₀ σ ss₁ σ' →
+  EvalStatements π δ δP σ₀ σ' ss₂ σ'' →
+  EvalStatements π δ δP σ₀ σ (ss₁ ++ ss₂) σ'' := by
+  apply Nat.strongRecOn
+    (motive := λ m ↦
+      ∀ ss₁ ss₂ σ σ' σ'',
+      sizeOf (ss₁ ++ ss₂) = m →
+      EvalStatements π δ δP σ₀ σ ss₁ σ' →
+      EvalStatements π δ δP σ₀ σ' ss₂ σ'' →
+      EvalStatements π δ δP σ₀ σ (ss₁ ++ ss₂) σ'')
+    (sizeOf (ss₁ ++ ss₂))
+  intros n ih ss₁ ss₂ σ σ' σ'' Hsize Heval1 Heval2
+  . cases Heval1 with
+    | stmts_none_sem => assumption
+    | stmts_some_sem Heval1 Heval1' =>
+      next s σ₁ ss =>
+      constructor <;> try assumption
+      simp [sizeOf] at *
+      have Hsz : Stmts.sizeOf (ss ++ ss₂) = n - 1 - s.sizeOf := by omega
+      apply ih _ (by omega) ss ss₂ σ₁ σ' σ'' Hsz
+      assumption
+      assumption
+  . rfl
+
+theorem HavocVarsApp :
+  HavocVars σ vs₁ σ' →
+  HavocVars σ' vs₂ σ'' →
+  HavocVars σ (vs₁ ++ vs₂) σ'' := by
+  intros Hv1 Hv2
+  induction vs₁ generalizing σ
+  case nil =>
+    simp
+    have Heq := HavocVarsEmpty Hv1
+    simp [Heq]
+    assumption
+  case cons h t ih =>
+    simp
+    cases Hv1
+    next exp σ1 Hup Hhavoc =>
+    apply HavocVars.update_some <;> try assumption
+    exact ih Hhavoc
+
+theorem HavocVarsApp' :
+  HavocVars σ (vs₁ ++ vs₂) σ'' →
+  ∃ σ',
+  HavocVars σ vs₁ σ' ∧
+  HavocVars σ' vs₂ σ'' := by
+  intros Hv
+  induction vs₁ generalizing σ
+  case nil =>
+    exists σ
+    simp_all
+    constructor
+  case cons h t ih =>
+    cases Hv
+    next exp σ1 Hup Hhavoc =>
+    specialize ih Hhavoc
+    cases ih with
+    | intro σ₁ Hand =>
+    cases Hand with
+    | intro Havoc1 Havoc2 =>
+    exists σ₁
+    simp_all
+    constructor <;> assumption
+
+theorem InitVarsApp :
+  InitVars σ vs₁ σ' →
+  InitVars σ' vs₂ σ'' →
+  InitVars σ (vs₁ ++ vs₂) σ'' := by
+  intros Hv1 Hv2
+  induction vs₁ generalizing σ
+  case nil =>
+    simp
+    have Heq := InitVarsEmpty Hv1
+    simp [Heq]
+    assumption
+  case cons h t ih =>
+    simp
+    cases Hv1
+    next exp σ1 Hup Hhavoc =>
+    apply InitVars.init_some <;> try assumption
+    exact ih Hhavoc
+
+theorem TouchVarsApp :
+  TouchVars σ vs₁ σ' →
+  TouchVars σ' vs₂ σ'' →
+  TouchVars σ (vs₁ ++ vs₂) σ'' := by
+  intros Hv1 Hv2
+  induction vs₁ generalizing σ
+  case nil =>
+    simp
+    have Heq := TouchVarsEmpty Hv1
+    simp [Heq]
+    assumption
+  case cons h t ih =>
+    simp
+    cases Hv1 with
+    | init_some Hinit Htouch =>
+      exact TouchVars.init_some Hinit (ih Htouch)
+    | update_some Hup Htouch =>
+      exact TouchVars.update_some Hup (ih Htouch)
+
+theorem HavocVarsCons :
+  HavocVars σ [v] σ' →
+  HavocVars σ' vs σ'' →
+  HavocVars σ (v :: vs) σ'' := by
+  intros Hv1 Hv2
+  have Heq : (v :: vs = [v] ++ vs) := by rfl
+  rw [Heq]
+  exact HavocVarsApp Hv1 Hv2
+
+theorem HavocVarsId :
+  isDefined σ vs →
+  HavocVars σ vs σ := by
+  intros Hdef
+  induction vs
+  constructor
+  next P h t ih =>
+  have Hh := Hdef h List.mem_cons_self
+  simp [Option.isSome] at Hh
+  split at Hh <;> simp_all
+  next x v' heq =>
+  apply @HavocVars.update_some (σ':=σ) (v:=v')
+  exact UpdateState.update heq heq fun y => congrFun rfl
+  apply ih
+  simp [isDefined] at *
+  intros v Hin
+  apply Hdef.2 v Hin
+
+theorem TouchVarsId :
+  isDefined σ vs →
+  TouchVars σ vs σ := by
+  intros Hdef
+  induction vs
+  constructor
+  next P h t ih =>
+  have Hh := Hdef h List.mem_cons_self
+  simp [Option.isSome] at Hh
+  split at Hh <;> simp_all
+  next x v' heq =>
+  apply @TouchVars.update_some (σ':=σ) (v:=v')
+  exact UpdateState.update heq heq fun y => congrFun rfl
+  apply ih
+  simp [isDefined] at *
+  intros v Hin
+  apply Hdef.2 v Hin
+
+theorem InitStateDefMonotone
+  {P : PureExpr} {σ σ' : SemanticStore P}
+  {vs : List P.Ident} {e : P.Expr} {v : P.Ident} :
+  isDefined σ vs →
+  InitState P σ v e σ' →
+  isDefined σ' vs := by
+  intros Hdef Heval
+  cases Heval with
+  | init Hold HH Hsome =>
+  simp [isDefined] at *
+  intros v' Hv'
+  by_cases Heq: (v = v')
+  case pos =>
+    simp [Option.isSome]
+    simp [Heq] at *
+    split <;> simp_all
+  case neg =>
+    specialize Hsome v' Heq
+    specialize Hdef v'
+    simp [Hsome]
+    exact Hdef Hv'
+
+theorem InitStatesDefMonotone :
+  isDefined σ vs →
+  InitStates σ vs' es' σ' →
+  isDefined σ' vs := by
+  intros Hdef Hhavoc
+  induction Hhavoc with
+  | init_some Hup Hhav ih =>
+  apply ih
+  apply InitStateDefMonotone <;> assumption
+  | init_none => simp_all
+
+theorem InitVarsDefMonotone :
+  isDefined σ vs →
+  InitVars σ vs' σ' →
+  isDefined σ' vs := by
+  intros Hdef Hhavoc
+  induction Hhavoc with
+  | init_some Hup Hhav ih =>
+  apply ih
+  apply InitStateDefMonotone <;> assumption
+  | init_none => simp_all
+
+theorem InitStateDefMonotone'
+  {P : PureExpr} {σ σ' : SemanticStore P}
+  {vs : List P.Ident} {e : P.Expr} {v : P.Ident} :
+  ¬ v ∈ vs →
+  isDefined σ' vs →
+  InitState P σ v e σ' →
+  isDefined σ vs := by
+  intros Hnin Hdef Heval
+  cases Heval with
+  | init Hold HH Hsome =>
+  simp [isDefined] at *
+  intros v' Hv'
+  by_cases Heq: (v = v')
+  case pos =>
+    simp [Option.isSome]
+    simp [Heq] at *
+    split <;> simp_all
+  case neg =>
+    specialize Hsome v' Heq
+    specialize Hdef v'
+    simp [← Hsome]
+    exact Hdef Hv'
+
+theorem InitStatesDefMonotone' :
+  vs.Disjoint vs' →
+  isDefined σ' vs →
+  InitStates σ vs' es' σ' →
+  isDefined σ vs := by
+  intros Hdisj Hdef Hhavoc
+  induction Hhavoc with
+  | init_none => assumption
+  | init_some Hup Hhav ih =>
+  next σ x v σ' xs' ys' σ'' =>
+  apply InitStateDefMonotone' (σ':=σ') <;> try assumption
+  . intros Hin
+    apply Hdisj Hin
+    exact List.mem_cons_self
+  . apply ih
+    . apply List.Disjoint.mono_right _ Hdisj
+      exact List.sublist_cons_self x xs'
+    . assumption
+
+theorem InitVarsDefMonotone' :
+  vs.Disjoint vs' →
+  isDefined σ' vs →
+  InitVars σ vs' σ' →
+  isDefined σ vs := by
+  intros Hdisj Hdef Hinit
+  have Hinit := InitVarsInitStates Hinit
+  cases Hinit with
+  | intro es Hinit =>
+  exact InitStatesDefMonotone' Hdisj Hdef Hinit
+
+theorem InitStatesDefined :
+  InitStates σ hs vs σ' → isDefined σ' hs := by
+  intros Hinit
+  induction Hinit <;> simp [isDefined]
+  case init_some x v σ' xs vs σ'' Hinit Hinits ih =>
+    simp [isDefined] at *
+    cases Hinit with
+    | init Hnone Hsome Heq =>
+    refine ⟨?_, by simp_all⟩
+    have Hdef : isDefined σ'' [x] := by
+      apply InitStatesDefMonotone ?_ Hinits
+      simp [isDefined, Option.isSome]
+      split <;> simp_all
+    simp [isDefined] at Hdef
+    assumption
+
+theorem HavocVarsDefMonotone :
+  isDefined σ vs →
+  HavocVars σ vs' σ' →
+  isDefined σ' vs := by
+  intros Hdef Hhavoc
+  induction Hhavoc with
+  | update_some Hup Hhav ih =>
+  apply ih
+  apply UpdateStateDefMonotone <;> assumption
+  | update_none => simp_all
+
+theorem HavocVarsUpdateStates : HavocVars σ vars σ' →
+  ∃ modvals, UpdateStates σ vars modvals σ' := by
+  intros Hhav
+  induction Hhav
+  case update_none =>
+    refine ⟨[], UpdateStates.update_none⟩
+  case update_some σ x v σ₁ xs σ'' Hup Hhav Hex =>
+    cases Hex with
+    | intro vs Hups =>
+    refine ⟨v::vs,?_⟩
+    constructor <;> assumption
+
+theorem HavocVarsDefMonotone' :
+  isDefined σ' vs →
+  HavocVars σ vs' σ' →
+  isDefined σ vs := by
+  intros Hdef Hhavoc
+  have Hup := HavocVarsUpdateStates Hhavoc
+  cases Hup with
+  | intro es Hinit =>
+  exact UpdateStatesDefMonotone' Hdef Hinit
+
+theorem InitVarsDefined :
+  InitVars σ vs σ' →
+  isDefined σ' vs := by
+  intros Hhavoc
+  induction vs generalizing σ σ'
+  case nil => simp [isDefined]
+  case cons h t ih =>
+    cases Hhavoc with
+    | @init_some _ _ v σ₁ _ _ Hup Hhav =>
+    apply isDefinedCons
+    apply InitVarsDefMonotone (σ:=σ₁)
+    apply InitStateDefined <;> assumption
+    assumption
+    apply ih <;> assumption
+
+theorem InitVarsReadValues :
+  InitVars σ ks σ' →
+  exists vs,
+  ReadValues σ' ks vs := by
+  intros Hinit
+  induction Hinit
+  case init_none =>
+    exists []
+    constructor
+  case init_some x x' σ xs σ' Hinit Hinits ih =>
+  cases Hinit with
+  | init Hnone Hsome Hinv =>
+  cases ih with
+  | intro xs' Hrds =>
+  exists x' :: xs'
+  constructor <;> simp_all
+  have Hrd : ReadValues σ [x] [x'] :=
+    ReadValues.read_some Hsome ReadValues.read_none
+  have Hrd' := InitVarsReadValuesMonotone Hrd Hinits
+  cases Hrd'
+  assumption
+
+theorem HavocVarsDefined :
+  HavocVars σ vs σ' →
+  isDefined σ' vs := by
+  intros Hhavoc
+  induction vs generalizing σ σ'
+  case nil => simp [isDefined]
+  case cons h t ih =>
+    cases Hhavoc with
+    | @update_some _ _ v σ₁ _ _ Hup Hhav =>
+    apply isDefinedCons
+    apply HavocVarsDefMonotone (σ:=σ₁)
+    apply UpdateStateDefined <;> assumption
+    assumption
+    apply ih <;> assumption
+
+theorem EvalCmdDefMonotone :
+  isDefined σ v →
+  EvalCmd Boogie.Expression δ δP σ₀ σ c σ' →
+  isDefined σ' v := by
+  intros Hdef Heval
+  cases Heval <;> try exact Hdef
+  next _ _ Hup => exact InitStateDefMonotone Hdef Hup
+  next _ _ Hup => exact UpdateStateDefMonotone Hdef Hup
+  next _ _ Hup => exact UpdateStateDefMonotone Hdef Hup
+
+theorem EvalCmdTouch
+  [HasVal P] [HasFvar P] [HasBool P] [HasBoolVal P] [HasBoolNeg P] :
+  EvalCmd P δ δP σ₀ σ c σ' →
+  TouchVars σ (HasVarsImp.touchedVars c) σ' := by
+  intro Heval
+  induction Heval <;> simp [HasVarsImp.touchedVars, Cmd.definedVars, Cmd.modifiedVars]
+  case eval_init x' δ σ x v σ' δP σ₀ e Hsm Hup Hwf =>
+    apply TouchVars.init_some Hup
+    constructor
+  case eval_set δ σ x v σ' δP σ₀ e Hsm Hup Hwf =>
+    exact TouchVars.update_some Hup TouchVars.none
+  case eval_havoc x v σ' δP σ₀ e Hsm Hup Hwf =>
+    exact TouchVars.update_some Hup TouchVars.none
+  case eval_assert => exact TouchVars.none
+  case eval_assume => exact TouchVars.none
+
+theorem UpdateStatesHavocVars : UpdateStates σ vars modvals σ' → HavocVars σ vars σ' := by
+  intros H
+  induction vars generalizing σ modvals
+  case nil =>
+    cases modvals
+    . have Heq := UpdateStatesEmpty H
+      simp [Heq]
+      apply HavocVars.update_none
+    . cases H
+  case cons h t ih =>
+    have HH := H
+    cases H
+    next Hup2 =>
+    constructor <;> try assumption
+    apply ih
+    apply Hup2
+
+theorem UpdateStatesTouchVars : UpdateStates σ vars modvals σ' → TouchVars σ vars σ' := by
+  intros H
+  induction vars generalizing σ modvals
+  case nil =>
+    cases modvals
+    . have Heq := UpdateStatesEmpty H
+      simp [Heq]
+      apply TouchVars.none
+    . cases H
+  case cons h t ih =>
+    have HH := H
+    cases H
+    next Hup2 =>
+    apply TouchVars.update_some <;> try assumption
+    apply ih
+    apply Hup2
+
+theorem EvalCmdRefinesContract :
+EvalCmd Expression δ δP σ₀ σ c σ' →
+EvalCommandContract π δ δP σ₀ σ (CmdExt.cmd c) σ' := by
+intros H; constructor; assumption
+
+theorem InvStoresUpdatedStateDisjRightMono :
+  ¬ k' ∈ ks →
+  invStores σ σ' ks →
+  invStores σ (updatedState σ' k' v') ks := by
+  intros Hnin Hinv
+  induction ks generalizing k' v'
+  case nil =>
+    intros k1 k2 Hin
+    cases Hin
+  case cons h t ih =>
+    intros k1 k2 Hin
+    simp_all
+    cases Hin
+    case inl H =>
+      simp [updatedState]
+      split <;> simp_all
+      apply Hinv
+      exact List.mem_of_mem_head? rfl
+    case inr H =>
+      apply ih Hnin.2
+      intros k1 k2 Hin
+      apply Hinv
+      exact List.mem_of_mem_tail Hin
+      exact H
+
+theorem InvStoresUpdatedStatesDisjRightMono :
+  ks.Disjoint ks' →
+  invStores σ σ' ks →
+  ks'.length = vs'.length →
+  invStores σ (updatedStates σ' ks' vs') ks := by
+  intros Hdis Hinv Hlen k1 k2 Hin
+  simp [updatedStates]
+  simp [zip_self_eq Hin] at *
+  induction ks' generalizing vs' σ σ'
+  case nil =>
+    simp [updatedStates']
+    exact Hinv k2 k2 Hin
+  case cons h t ih =>
+    induction vs' generalizing h t σ σ' <;> simp_all
+    case cons h' t' ih' =>
+      simp [updatedStates']
+      rw [← ih] <;> try simp_all
+      . intros k Hin1 Hin2
+        apply Hdis Hin1
+        exact List.mem_cons_of_mem h Hin2
+      . refine InvStoresUpdatedStateDisjRightMono ?_ Hinv
+        intros Hin
+        exact Hdis Hin List.mem_cons_self
+
+theorem InvStoresUpdatedStateDisjLeftMono :
+  ¬ k' ∈ ks →
+  invStores σ σ' ks →
+  invStores (updatedState σ k' v') σ' ks := by
+  intros Hnin Hinv
+  have Hinv' := substStoresFlip Hinv
+  simp [invStores]
+  apply substStoresFlip'
+  simp [substSwap] at *
+  rw [← invStores]
+  exact InvStoresUpdatedStateDisjRightMono Hnin Hinv'
+
+theorem InvStoresUpdatedStatesDisjLeftMono :
+  ks.Disjoint ks' →
+  invStores σ σ' ks →
+  ks'.length = vs'.length →
+  invStores (updatedStates σ ks' vs') σ' ks := by
+  intros Hnin Hinv Hlen
+  have Hinv' := substStoresFlip Hinv
+  simp [invStores]
+  apply substStoresFlip'
+  simp [substSwap] at *
+  rw [← invStores]
+  apply InvStoresUpdatedStatesDisjRightMono Hnin Hinv' Hlen
+
+theorem InvStoresExceptEmpty : invStoresExcept σ σ [] :=
+  fun _ _ _ _ Hin => congrArg σ (zip_self_eq Hin)
+
+theorem InvStoresExceptId : invStoresExcept σ σ ls :=
+  fun _ _ _ _ Hin => congrArg σ (zip_self_eq Hin)
+
+theorem InvStoresExceptApp :
+  invStoresExcept σ σ' ks →
+  invStoresExcept σ σ' (ks ++ ks') := by
+  intros Hinv x Hdisj
+  apply Hinv
+  exact List.DisjointAppRight' Hdisj
+
+theorem InvStoresExceptUpdated :
+  invStoresExcept σ σ' ks →
+  ks'.length = vs'.length →
+  invStoresExcept (updatedStates σ ks' vs') σ' (ks ++ ks') := by
+  intros Hinv Hlen
+  simp [invStoresExcept] at *
+  intros vsInv Hdisj
+  refine InvStoresUpdatedStatesDisjLeftMono ?_ ?_ Hlen
+  exact List.DisjointAppLeft' Hdisj
+  apply Hinv
+  exact List.DisjointAppRight' Hdisj
+
+theorem UpdatedStatesInSame :
+  k ∈ ks' →
+  ks'.length = vs'.length →
+  ks'.Nodup →
+  updatedStates σ ks' vs' k = updatedStates σ' ks' vs' k := by
+  intros Hin Hlen Hnd
+  induction ks' generalizing vs' k σ σ' <;>
+    simp [updatedStates, updatedStates'] <;> simp_all
+  case cons h t ih =>
+    cases vs'
+    case nil => simp_all
+    case cons =>
+    simp [updatedStates']
+    cases Hin with
+    | inl Heq =>
+      simp_all
+      rw [← updatedStateComm']
+      rw [← updatedStateComm']
+      simp [updatedState]
+      . simp_all
+        intros x Hin
+        have HH := List.of_mem_zip Hin
+        simp_all
+      . simp_all
+        intros x Hin
+        have HH := List.of_mem_zip Hin
+        simp_all
+    | inr Hin =>
+      apply ih <;> simp_all
+
+theorem UpdatedStatesNotinSame :
+  σ k = σ' k →
+  ¬ k ∈ ks' →
+  ks'.length = vs'.length →
+  ks'.Nodup →
+  updatedStates σ ks' vs' k = updatedStates σ' ks' vs' k := by
+  intros Heq Hnin Hlen Hnd
+  induction ks' generalizing vs' k σ σ' <;>
+    simp [updatedStates, updatedStates'] <;> simp_all
+  case cons h t ih =>
+    cases vs'
+    case nil => simp_all
+    case cons =>
+    simp [updatedStates']
+    rw [← updatedStateComm']
+    rw [← updatedStateComm']
+    . simp [updatedState]
+      split <;> simp_all
+      apply ih <;> simp_all
+    . simp_all
+      intros x Hin
+      have HH := List.of_mem_zip Hin
+      simp_all
+    . simp_all
+      intros x Hin
+      have HH := List.of_mem_zip Hin
+      simp_all
+
+theorem InvStoresExceptUpdatedSame :
+  invStoresExcept σ σ' ks →
+  ks'.length = vs'.length →
+  ks'.Nodup →
+  invStoresExcept (updatedStates σ ks' vs') (updatedStates σ' ks' vs') ks := by
+  intros Hinv Hlen Hnd
+  simp [invStoresExcept] at *
+  intros vsInv Hdisj k1 k2 Hin
+  have Heq := zip_self_eq Hin
+  simp [Heq]
+  by_cases Hin : k2 ∈ ks'
+  case pos =>
+    exact UpdatedStatesInSame Hin Hlen Hnd
+  case neg =>
+    refine UpdatedStatesNotinSame ?_ Hin Hlen Hnd
+    apply Hinv _ Hdisj
+    simp_all
+
+theorem InvStoresExceptUpdatedMem :
+  invStoresExcept σ σ' ks →
+  ks'.length = vs'.length →
+  ks'.Subset ks →
+  invStoresExcept (updatedStates σ ks' vs') σ' ks := by
+  intros Hinv Hlen
+  simp [invStoresExcept] at *
+  intros Hsub vs Hdisj
+  refine InvStoresUpdatedStatesDisjLeftMono ?_ ?_ Hlen
+  exact List.Disjoint_Subset Hdisj Hsub
+  exact Hinv _ Hdisj
+
+theorem InvStoresExceptUpdateStates :
+  invStoresExcept σ σ' ks →
+  UpdateStates σ ks' vs' σ'' →
+  invStoresExcept σ'' σ' (ks ++ ks') := by
+  intros Hinv Hup
+  have Hup' := UpdateStatesUpdated Hup
+  simp [Hup']
+  refine InvStoresExceptUpdated Hinv ?_
+  exact UpdateStatesLength Hup
+
+theorem InvStoresExceptInitStates :
+  invStoresExcept σ σ' ks →
+  InitStates σ ks' vs' σ'' →
+  invStoresExcept σ'' σ' (ks ++ ks') := by
+  intros Hinv Hup
+  have Hup' := InitStatesUpdated Hup
+  simp [Hup']
+  refine InvStoresExceptUpdated Hinv ?_
+  exact InitStatesLength Hup
+
+theorem InvStoresExceptHavocVars :
+  invStoresExcept σ σ' ks →
+  HavocVars σ ks' σ'' →
+  invStoresExcept σ'' σ' (ks ++ ks') := by
+  intros Hinv Hup
+  have Hup' := HavocVarsUpdateStates Hup
+  cases Hup' with
+  | intro vs' Hups =>
+  exact InvStoresExceptUpdateStates Hinv Hups
+
+theorem InvStoresExceptInitVars :
+  invStoresExcept σ σ' ks →
+  InitVars σ ks' σ'' →
+  invStoresExcept σ'' σ' (ks ++ ks') := by
+  intros Hinv Hup
+  have Hup' := InitVarsInitStates Hup
+  cases Hup' with
+  | intro vs' Hups =>
+  exact InvStoresExceptInitStates Hinv Hups
+
+theorem InvStoresExceptInvStores :
+  invStoresExcept σ σ' ks →
+  List.Disjoint ks ks' →
+  invStores σ σ' ks' := by
+  intros Hinv Hdis k1 k2 Hin
+  apply Hinv ks'
+  exact List.Disjoint.symm Hdis
+  assumption
+
+set_option warn.sorry false in
+/--
+Note: Currently we cannot prove this theorem,
+  since `WellFormedSemanticEval` definition does not assert
+  a congruence relation for definedness on store,
+  that is, if `f(a)` is defined, then `a` must be defined.
+  We work around this by requiring this condition at `EvalExpressions`.
+  -/
+theorem EvalExpressionIsDefined :
+  WellFormedBoogieEvalCong δ →
+  WellFormedSemanticEvalVar δ →
+  (δ σ₀ σ e).isSome →
+  isDefined σ (HasVarsPure.getVars e) := by
+  intros Hwfc Hwfvr Hsome
+  intros v Hin
+  simp [WellFormedBoogieEvalCong] at Hwfc
+  simp [WellFormedSemanticEvalVar] at Hwfvr
+  induction e generalizing v <;>
+    simp [HasVarsPure.getVars, Lambda.LExpr.LExpr.getVars] at *
+  case fvar v' ty' =>
+    specialize Hwfvr (Lambda.LExpr.fvar v' ty') v' σ₀ σ
+    simp [HasFvar.getFvar] at Hwfvr
+    simp_all
+  case mdata info e ih =>
+    -- Need extra congruence properties -- if f(a) is defined, then a must be defined
+    sorry
+  case abs => sorry
+  case quant => sorry
+  case app => sorry
+  case ite => sorry
+  case eq => sorry
+
+set_option warn.sorry false in
+/--
+NOTE:
+  In order to prove this refinement theorem, we need to reason about the
+  assymmetry between the two semantics regarding the temporary variables
+  created in the concrete semantics. That is, evaluating the procedure body may
+  create new variables in the store, and since the temporary variables are
+  discarded at the end of the call, it is possible to show that those created
+  variables are irrelevant, and can be approximated by updating the relevant
+  variables (that is, lhs ++ modifies)
+-/
+theorem EvalCallBodyRefinesContract :
+  ∀ {π δ δP σ₀ σ lhs n args σ' p},
+  π n = .some p →
+  p.spec.modifies = Imperative.HasVarsTrans.modifiedVarsTrans π p.body →
+  EvalStatement π δ δP σ₀ σ (.call lhs n args) σ' →
+  EvalStatementContract π δ δP σ₀ σ (.call lhs n args) σ' := by
+  intros π δ δP σ₀ σ lhs n args σ' p pFound modValid H
+  cases H with
+  | cmd_sem Heval Hdef =>
+    cases Heval with
+    | call_sem lkup Heval Hwfval Hwfvars Hwfb Hwf Hwf2 Hup Hhav Hpre Heval2 Hpost Hrd Hup2 =>
+      sorry
