Strata/DL/Util/LabelGen.lean
@@ -1,0 +1,60 @@
+/-
+  Copyright Strata Contributors
+
+  SPDX-License-Identifier: Apache-2.0 OR MIT
+-/
+
+import Strata.DL.Util.Counter
+import Strata.DL.Util.StringGen
+namespace LabelGen
+
+/--
+a label generator of type α,
+  guaranteeing that all generated labels are unique
+  -/
+class WFLabelGen (α : Type) (State : Type) [HasSubset State] [DecidableEq α] where
+  /-- an empty state -/
+  emp : State
+  /-- a generator function -/
+  gen : α → State → (α × State)
+  /-- all labels generated so far -/
+  generated : State → List α
+  wf : State → Prop
+  wf_emp : wf emp
+  wf_gen : ∀ (γ γ': State) (pf l: α),
+    gen pf γ = (l, γ') →
+    wf γ →
+    wf γ' ∧ l ∈ generated γ' ∧ γ ⊆ γ'
+
+/-- CounterState has a unique generator -/
+instance : WFLabelGen Nat Counter.CounterState where
+  emp := Counter.CounterState.emp
+  gen := λ _ ↦ Counter.genCounter -- discards the prefix
+  generated := Counter.CounterState.generated
+  wf := Counter.WF
+  wf_emp := by
+    constructor ; simp [Counter.CounterState.emp] ; simp
+  wf_gen := fun γ γ' _ l Hgen Hwf =>
+    ⟨Counter.genCounterWFMono Hwf Hgen,
+    Counter.genCounterContains Hgen,
+    Counter.genCounterSubset Hgen⟩
+
+
+/-- StringGen has a unique generator -/
+instance : WFLabelGen String StringGenState where
+  emp := .emp
+  gen := StringGenState.gen
+  generated := Prod.snd ∘ List.unzip ∘ StringGenState.generated
+  wf := StringGenState.WF
+  wf_emp := by
+    simp [StringGenState.WF, Counter.WF]
+  wf_gen := by
+    intros γ γ' pf l Hgen Hwf
+    refine ⟨?_, ?_, ?_⟩
+    . exact StringGenState.WFMono Hwf Hgen
+    . exact StringGenState.contains Hgen
+    . exact StringGenState.subset Hgen
+
+abbrev StringGenM := StateM StringGenState
+
+end LabelGen
